Some messy suprema proofs

OmniaLib/Order/Relation/Defs.lean
@@ -18,29 +18,41 @@ trans : ∀ (a b c : α), a ∈ S → b ∈ S → c ∈ S →  r a b → r b c �
 class total (α : Type u) (r : α → α → Prop) (S : set α) : Prop where
 total : ∀ (a b : α), a ∈ S → b ∈ S → r a b ∨ r b a
 
-class has_bot (α : Type u) (r : α → α → Prop) (S : set α) where
+class bot (α : Type u) where
 bot : α
-bot_mem : bot ∈ S
-bot_def : ∀ (a : α), a ∈ S → r bot a
+notation "⊥" => bot.bot
 
-class has_top (α : Type u) (r : α → α → Prop) (S : set α) : Type u where
+class top (α : Type u) where
 top : α
-top_mem : top ∈ S
-top_def : ∀ (a : α), a ∈ S → r a top
+notation "⊤" => top.top
 
-class has_inf (α : Type u) (r : α → α → Prop) (S : set α) : Type u where
+class inf (α : Type u) where
 inf : α → α → α
-inf_mem : ∀ (a b : α), a ∈ S → b ∈ S → inf a b ∈ S
-inf_left : ∀ (a b : α), a ∈ S → b ∈ S → r (inf a b) a
-inf_right : ∀ (a b : α), a ∈ S → b ∈ S → r (inf a b) b
-inf_higher : ∀ (a b c : α), a ∈ S → b ∈ S → c ∈ S → r c a → r c b → r c (inf a b)
+infix:80 " ⊓ " => inf.inf
 
-class has_sup (α : Type u) (r : α → α → Prop) (S : set α) : Type u where
+class sup (α : Type u) where
 sup : α → α → α
-sup_mem : ∀ (a b : α), a ∈ S → b ∈ S → sup a b ∈ S
-sup_left : ∀ (a b : α), a ∈ S → b ∈ S → r a (sup a b)
-sup_right : ∀ (a b : α), a ∈ S → b ∈ S → r b (sup a b)
-sup_lower : ∀ (a b c : α), a ∈ S → b ∈ S → c ∈ S → r a c → r b c → r (sup a b) c
+infix:80 " ⊔ " => sup.sup
+
+class has_bot (α : Type u) (r : α → α → Prop) (S : set α) extends bot α where
+bot_mem : ⊥ ∈ S
+bot_def : ∀ (a : α), a ∈ S → r ⊥ a
+
+class has_top (α : Type u) (r : α → α → Prop) (S : set α) extends top α where
+top_mem : ⊤ ∈ S
+top_def : ∀ (a : α), a ∈ S → r a ⊤
+
+class has_inf (α : Type u) (r : α → α → Prop) (S : set α) extends inf α where
+inf_mem : ∀ (a b : α), a ∈ S → b ∈ S → a ⊓ b ∈ S
+inf_left : ∀ (a b : α), a ∈ S → b ∈ S → r (a ⊓ b) a
+inf_right : ∀ (a b : α), a ∈ S → b ∈ S → r (a ⊓ b) b
+inf_higher : ∀ (a b c : α), a ∈ S → b ∈ S → c ∈ S → r c a → r c b → r c (a ⊓ b)
+
+class has_sup (α : Type u) (r : α → α → Prop) (S : set α) extends sup α where
+sup_mem : ∀ (a b : α), a ∈ S → b ∈ S → a ⊔ b ∈ S
+sup_left : ∀ (a b : α), a ∈ S → b ∈ S → r a (a ⊔ b)
+sup_right : ∀ (a b : α), a ∈ S → b ∈ S → r b (a ⊔ b)
+sup_lower : ∀ (a b c : α), a ∈ S → b ∈ S → c ∈ S → r a c → r b c → r (a ⊔ b) c
 
 -- basic structures studied in order theory
 class preorder (α : Type u) (r : α → α → Prop) (S : set α)
