OmniaLib/Order/Relation/Basic.lean
@@ -3,12 +3,41 @@ import OmniaLib.Order.Relation.Defs
 open Order
 
 theorem bot.unique (p₁ : has_bot α r A) (p₂ : antisymmetric α r A) :
-  ∀ (a : α), a ∈ A → r a p₁.bot → a = p₁.bot := by
+  ∀ (a : α), a ∈ A → r a ⊥ → a = ⊥ := by
 intro a ha hr
-have : r p₁.bot a := p₁.bot_def a ha
+have : r ⊥ a := p₁.bot_def a ha
 exact p₂.antisymm a p₁.bot ha p₁.bot_mem hr this
 
-theorem bot.inf_idemp (p : bounded_lattice α r A) : ∀ (a : α), a ∈ A → p.inf p.bot a = p.bot := by
+theorem bot.inf_idemp (p : bounded_lattice α r A) : ∀ (a : α), a ∈ A → ⊥ ⊓ a = ⊥ := by
 intro a ha
-have : r (p.inf p.bot a) p.bot := sorry
+have : r (⊥ ⊓ a) ⊥ := p.inf_left p.bot a p.bot_mem ha
+apply bot.unique p.tohas_bot p.toantisymmetric
+exact p.inf_mem p.bot a p.bot_mem ha
+exact this
+
+
+theorem dodo (p : lattice α r A) : ∀ (a : α), a ∈ A → a ⊔ a = a := by
+intro a ha
+apply p.antisymm
 sorry
+exact ha
+exact p.sup_lower a a a ha ha ha (p.refl a ha) (p.refl a ha)
+
+
+theorem doo (p : lattice α r A) : ∀ (a b : α), a ∈ A → b ∈ A → r a b → r (a ⊔ b) b := by
+intro a b ha hb rab
+exact p.sup_lower a b b ha hb hb rab (p.refl b hb)
+
+
+theorem bot.sup_idemp (p : bounded_lattice α r A) : ∀ (a : α), a ∈ A → ⊥ ⊔ a = a := by
+intro a ha
+apply p.antisymm _ _ (p.sup_mem p.bot a p.bot_mem ha) ha
+have : r (⊥ ⊔ a) a := by
+  apply doo
+  exact p.bot_mem
+  exact ha
+  exact p.bot_def a ha
+exact this
+apply p.sup_right ⊥ a
+exact p.bot_mem
+exact ha
